$\log_{2x}(48\sqrt[3]3)=\log_{3x}(162\sqrt[3]2)$

$\large{\ln(48\sqrt[3]3)\over \ln(2x)}={\ln(162\sqrt[3]2)\over \ln(3x)}$

Suppose $u=\ln(x)$, then $\ln(3x)=\ln3+u$, $\ln(2x)=\ln2+u$.

Therefore, ${u+\ln2\over \ln(16)+\ln(3\sqrt[3]3)}={u+\ln3\over \ln(81)+\ln(2\sqrt[3]2)}$.

${u+\ln2\over 4\ln2+{4\over 3} \ln3} ={u+\ln3\over 4\ln3+{4\over 3}\ln2}$

$(u+\ln2)(4\ln3+{4\over 3}\ln2)=(4\ln2+{4\over 3} \ln3)(u+\ln3)$

${8\over 3}(\ln3-\ln2)u={4\over 3}(\ln3-\ln2)(\ln3+\ln2)$

Therefore, $u={\ln3+\ln2\over 2}$.

Therefore, $x=e^u=e^{\ln3+\ln2\over 2}=e^{\ln3\over 2}\times e^{\ln2\over 2}=\sqrt 6$.